\documentclass{article}
\usepackage[margin=1cm]{geometry}
\usepackage{bm}

\usepackage{amsmath}
\usepackage{fontspec}
\setmainfont{FandolSong-Regular.otf}

\newcommand\D[1]{\Delta{#1}}
\newcommand\F[2]{\frac{#1}{#2}}
\newcommand\di[1]{\text{d}#1}

\begin{document}
  线性微分方程 常数变易法
  \begin{gather*}
    y = Y(x) \qquad u(x) = \frac{Q(x)}{Y(x)} \qquad v(x) = e^{\int u(x)\di{x}}\\
    \begin{aligned}
      \frac{\di{y}}{\di{x}} &= Q(x) - P(x)y \\
      &= Q(x) - P(x)Y(x) \\
      \frac{\di{y}}{Y(x)} &=  \left( \frac{Q(x)}{Y(x)} - P(x) \right)\di{x} \\
      \int\frac{1}{Y(x)}\di{y} &= \int\left(u(x) - P(x)\right)\di{x} \\
      \ln{y} &= \int\left(u(x) - P(x)\right)\di{x}\\
      y &= e^{\int u(x)\di{x} -\int P(x)\di{x}} \\
      &= e^{\int u(x)\di{x}} \times e^{-\int P(x)\di{x}} \\
      \frac{\di{y}}{\di{x}} &= v'(x)e^{-\int P(x)\di{x}} + v(x) \times -P(x)e^{-\int P(x)\di{x}} \\
      Q(x) - P(x)\left( e^{\int u(x)\di{x}} \times e^{-\int P(x)\di{x}} \right) &= v'(x)e^{-\int P(x)\di{x}} - v(x)P(x)e^{-\int P(x)\di{x}} \\
      Q(x) - v(x)P(x)e^{-\int P(x)\di{x}} &= v'(x)e^{-\int P(x)\di{x}} - v(x)P(x)e^{-\int P(x)\di{x}} \\
      Q(x) &= v'(x)e^{-\int P(x)\di{x}} \\
      \int Q(x)e^{\int P(x)\di{x}}\di{x} = \int \frac{Q(x)}{e^{-\int P(x)\di{x}}}\di{x} &= v(x) = e^{\int u(x)\di{x}} = \frac{y}{e^{-\int P(x)\di{x}}}  \\
      \int Q(x)e^{\int P(x)\di{x}}\di{x} \times e^{-\int P(x)\di{x}} &= y 
    \end{aligned} \\
  \end{gather*}
  \begin{align*}
    F\left(x\right) &= \int_{x}^{a} f\left(\frac{x}{2}\right) \,dx \\
    F'\left(x\right) &= \int_{x}^{a} f\left(\frac{x}{2}\right) \,dx
                        -\int_{x + \Delta{x}}^{a} f\left(\frac{x}{2}\right) \,dx
  \end{align*}
\end{document}