\documentclass{article}

\usepackage[margin=1cm]{geometry}
\usepackage{amsmath}
\usepackage{fontspec}
\setmainfont{FandolSong-Regular.otf}

\newcommand\D[1]{\Delta{#1}}
\newcommand\F[2]{\frac{#1}{#2}}
\newcommand\di[1]{\text{d}#1}

\begin{document}
  \begin{gather*}
    \begin{aligned}
      f(\alpha) =& 4 - ( A - \frac{\frac{2}{\cos(\alpha)}-2}{\tan(\alpha)} ) \tan(\alpha) \\
      =&4 - A\tan(\alpha) + \frac{2}{\cos(\alpha)}-2 \\
      =&2- A\tan(\alpha) + \frac{2}{\cos(\alpha)} \\
      g(\alpha) =& \frac{2 - f(\alpha)}{\tan(\alpha)} \\
      h(\alpha) =& A - g(\alpha) \\
      j(\alpha) =& h(\alpha) \cos(\alpha) \\
      k(\alpha) =& 2 \tan(\alpha) \\
      y(\alpha) =& j(\alpha) - k(\alpha) \\
      z(\alpha) =& y(\alpha) + ( 2 - f(\alpha) )\sin(\alpha) + g(\alpha)\sin(\alpha) \\
      =& j(\alpha) - k(\alpha) + (2-f(\alpha))\sin(\alpha) + \frac{2 - f(\alpha)}{\tan(\alpha)}\sin(\alpha) \\
      =& h(\alpha)\cos(\alpha) - 2\tan(\alpha) + (2-f(\alpha))\sin(\alpha) + (2 - f(\alpha))\cos(\alpha) \\
      =& (A-\frac{2 - f(\alpha)}{\tan(\alpha)})\cos(\alpha) - 2\tan(\alpha) + (2-f(\alpha))(\sin(\alpha)+\cos(\alpha)) \\
      =& A\cos(\alpha)-(2 - f(\alpha))\frac{\cos(\alpha)}{\tan(\alpha)} - 2\tan(\alpha) + (2-f(\alpha))(\sin(\alpha)+\cos(\alpha)) \\
      =& A\cos(\alpha)- 2\tan(\alpha) - (2-f(\alpha))(\frac{\cos(\alpha)}{\tan(\alpha)} - \sin(\alpha)-\cos(\alpha)) \\
      =& A\cos(\alpha)- 2\tan(\alpha) - (2-(2- A\tan(\alpha) + \frac{2}{\cos(\alpha)}))(\frac{\cos(\alpha)}{\tan(\alpha)} - \sin(\alpha)-\cos(\alpha)) \\
      =& A\cos(\alpha)- 2\tan(\alpha) - (A\tan(\alpha) - \frac{2}{\cos(\alpha)})(\frac{\cos^2(\alpha)}{\sin(\alpha)} - \sin(\alpha)-\cos(\alpha)) \\
      =& A\cos(\alpha)- 2\tan(\alpha) - A\cos(\alpha) + A\tan(\alpha)\sin(\alpha) + A\sin(\alpha) + \frac{2\cos(\alpha)}{\sin(\alpha)}-2\tan(\alpha)-2 \\
      =& - 2\tan(\alpha) + A\tan(\alpha)\sin(\alpha) + A\sin(\alpha) + \frac{2\cos(\alpha)}{\sin(\alpha)}-2\tan(\alpha)-2
      a
    \end{aligned}
  \end{gather*}
  \begin{gather*}
    \begin{aligned}
      f(\alpha) =&\frac{\frac{2}{\cos(\alpha)}-2}{\tan(\alpha)} \\
      =&\frac{\cos(\alpha)(\frac{2}{\cos(\alpha)}-2)}{\sin(\alpha)} \\
      =&\frac{2-2\cos(\alpha)}{\sin(\alpha)} \\
      f'(\alpha) =&\frac{(2-2\cos(\alpha))'\sin(\alpha) - (2-2\cos(\alpha))(\sin(\alpha))'}{\sin^2(\alpha)} \\
      =&\frac{(0-2(-\sin(\alpha)))\sin(\alpha)-(2-2\cos(\alpha))\cos(\alpha)}{\sin^2(\alpha)} \\
      =&\frac{2\sin^2(\alpha)-(2\cos(\alpha)-2\cos^2(\alpha))}{\sin^2(\alpha)} \\
      =&\frac{2\sin^2(\alpha)+2\cos^2(\alpha)-2\cos(\alpha)}{\sin^2(\alpha)} \\
      =&\frac{2-2\cos(\alpha)}{\sin^2(\alpha)}
    \end{aligned}
  \end{gather*}
  \begin{gather*}
    A = (a_{ij})_{m \times s} \\
    B = (b_{ij})_{s \times n} \\
    C = A \times B = (c_{ij})_{m \times n} \\
    c_{ij} = \sum_{k = 1}^{s} a_{ik}b_{kj} \\
    C = (c_{ij})_{n\times n} \\
    |C| = \sum -1^{\tau}c_{1j_{1}}\dots c_{nj_{n}}
  \end{gather*}
  \begin{gather*}
    \begin{aligned}
      k^3 - (k-1)^3 =& k^3 - \left(k^3 - 3k^2 + 3k -1\right) \\
      =& 3k^2 - 3k + 1 \\
      \sum_{k=1}^{n}k^3 - (k-1)^3 =& 3\sum_{k=1}^{n}k^2 - 3\sum_{k=1}^{n} k + n \\
      3\sum_{k=1}^{n}k^2 =& \sum_{k=1}^{n}k^3 - (k-1)^3 + 3\sum_{k=1}^{n} k - n \\
      =& n^3 + \frac{3n(n+1)}{2} - n \\
      =& \frac{2n^3 + 3n(n+1) - 2n}{2} \\
      =& \frac{2n^3 + 3n^2 + 3n - 2n}{2} \\
      =& \frac{2n^3 + 3n^2 + n}{2} \\
      =& \frac{n(2n^2 + 3n + 1)}{2} \\
      =& \frac{n(2n + 1)(n + 1)}{2}
    \end{aligned}
  \end{gather*}
  \begin{gather*}
    \frac{\di{y}}{\di{x}} - \frac{2y}{x + 1} = ( x + 1 )^{\frac{5}{2}} \\
    \frac{\di{y}}{\di{x}} = \frac{2y}{x + 1} \\
    \int\frac{\di{y}}{y} = \int\frac{2}{x + 1}\di{x} \\
    \ln{\left\lvert y\right\rvert} = 2\ln{\left\lvert x + 1\right\rvert} + C_1 \\
    y = C_1(x+1)^2 \\
    u'(x)(x+1)^2 + 2u(x)(x+1) = (x + 1)^{\frac{5}{2}} + \frac{2u(x)(x+1)^2}{x+1} \\
    u'(x) = \frac{(x+1)^{\frac{5}{2}}}{(x+1)^2} = (x+1)^{\frac{1}{2}} \\
    u(x) = \frac{3}{2}(x+1)^{\frac{3}{2}} + C \\
    y(x) = (\frac{3}{2}(x+1)^{\frac{3}{2}} + C)(x+1)^2
    % \int( x + 1 )^{\frac{5}{2}}e^{\int\frac{-2}{x + 1}\di{x}}\di{x} \times e^{-\int\frac{-2}{x + 1}\di{x}} = y \\
    % \int\frac{-2}{x+1} = -2\ln(x + 1) + C_1 \\
    % \begin{aligned}
    %   e^{\int\frac{-2}{x + 1}\di{x}}\di{x} &= e^{-2\ln(x + 1) + C_1} \\
    %   &= (e^{\ln(x + 1)})^{-2}e^{C_1} \\
    %   &= (x + 1)^{-2}e^{C_1}
    % \end{aligned} \\
    % \int( x + 1 )^{\frac{5}{2}}e^{-2\ln(x + 1) + C_1} \\
    % \int( x + 1 )^{\frac{5}{2}}(x + 1)^{-2} \times e^{C_1} \\
    % \left(\frac{2}{3}(x + 1)^{\frac{3}{2}} \times e^{C_1} + C_2\right) \times (x + 1)^2e^{C_3}
  \end{gather*}
  \begin{gather*}
    y = Y(x) \qquad u(x) = \frac{Q(x)}{Y(x)} \qquad v(x) = e^{\int u(x)\di{x}}\\
    \begin{aligned}
      \frac{\di{y}}{\di{x}} &= Q(x) - P(x)y \\
      &= Q(x) - P(x)Y(x) \\
      \frac{\di{y}}{Y(x)} &=  \left( \frac{Q(x)}{Y(x)} - P(x) \right)\di{x} \\
      \int\frac{1}{Y(x)}\di{y} &= \int\left(u(x) - P(x)\right)\di{x} \\
      \ln{y} &= \int\left(u(x) - P(x)\right)\di{x}\\
      y &= e^{\int u(x)\di{x} -\int P(x)\di{x}} \\
      &= e^{\int u(x)\di{x}} \times e^{-\int P(x)\di{x}} \\
      \frac{\di{y}}{\di{x}} &= v'(x)e^{-\int P(x)\di{x}} + v(x) \times -P(x)e^{-\int P(x)\di{x}} \\
      Q(x) - P(x)\left( e^{\int u(x)\di{x}} \times e^{-\int P(x)\di{x}} \right) &= v'(x)e^{-\int P(x)\di{x}} - v(x)P(x)e^{-\int P(x)\di{x}} \\
      Q(x) - v(x)P(x)e^{-\int P(x)\di{x}} &= v'(x)e^{-\int P(x)\di{x}} - v(x)P(x)e^{-\int P(x)\di{x}} \\
      Q(x) &= v'(x)e^{-\int P(x)\di{x}} \\
      \int Q(x)e^{\int P(x)\di{x}}\di{x} = \int \frac{Q(x)}{e^{-\int P(x)\di{x}}}\di{x} &= v(x) = e^{\int u(x)\di{x}} = \frac{y}{e^{-\int P(x)\di{x}}}  \\
      \int Q(x)e^{\int P(x)\di{x}}\di{x} \times e^{-\int P(x)\di{x}} &= y 
    \end{aligned} \\
  \end{gather*}
  \begin{gather*}
    y = ax \\
    y = bx \\
    (a\sin{C})^2 + (b-a\cos{C})^2 = c^2 \\
    a^2 - a^2\cos^2{C} + b^2 - 2ab\cos{C} + a^2\cos^2 = c^2 \\
    \cos{C} = \frac{a^2 + b^2 - c^2}{2ab}
  \end{gather*}
  \begin{gather*}
    u = \frac{x}{y} \\
    \begin{gathered}
      u = U(t) \quad x = X(t) \quad y = Y(t)
    \end{gathered} \\
    \begin{aligned}
      U(t) &= \F{Y(t)}{X(t)} \\
      \F{\di{U}(t)}{\di{t}} &= \left( \F{Y(t + \D{t})X(t) - Y(t)X(t + \D{t})}{X(t + \D{t})X(t)} \right) \F{1}{\D{t}} \\
      &= \F{Y'(t)X(t) - Y(t)X'(t)}{X^2(t)} \\
      \di{U}(t) &= \F{\di{Y}(t)X(t) - Y(t)\di{X}(t)}{X^2(t)} \\
      \di{u} & = \F{\di{y}x - \di{x}y}{x^{2}} \\
      \F{\di{u}}{\di{x}} &= \F{\di{y}}{\di{x}}\F{1}{x} - \F{y}{x^2} \\
      x\left( \F{\di{u}}{\di{x}} + \F{y}{x^2} \right) &= \F{\di{y}}{\di{x}} \\
      x\F{\di{u}}{\di{x}} + u &= \F{\di{y}}{\di{x}} \\
      \di{y} &= \di{u}x + u\di{x} \\
    \end{aligned} \\
    \begin{gathered}
      \ln{\F{y}{x}}\di{y} + \F{y}{x}\di{x} = 0 \\
    \end{gathered} \\
    \begin{aligned}
      \ln{u}(\di{u}x + u\di{x}) + u\di{x} &= 0 \\ 
      \ln{u}\di{u}x + ( \ln{u} + 1 ) u\di{x} &= 0 \\
      \ln{u}\di{u} + ( \ln{u} + 1 ) u\F{\di{x}}{x} &= 0 \\
      -\F{\di{x}}{x} = \F{\ln{u}}{\left( \ln{u} + 1 \right)u}\di{u}n
    \end{aligned}
  \end{gather*}
  \begin{gather*}
    ax^{2}+bx+c = 0 \\
    x^{2}+\frac{b}{a}x+\frac{c}{a} = 0 \\
    \begin{aligned}
      z+\frac{c}{a} =& \left(\frac{b}{2a}\right)^{2} \\
      z =& \left(\frac{b}{2a}\right)^{2} - \frac{c}{a} \\
    \end{aligned} \\
    \begin{aligned}
      \left(x + \frac{b}{2a}\right)^{2} - \left( \left(\frac{b}{2a}\right)^{2} - \frac{c}{a} \right) &= 0 \\
      \left(x + \frac{b}{2a}\right)^{2} &= \left( \left(\frac{b}{2a}\right)^{2} - \frac{c}{a} \right) \\
      x &= \pm\frac{\sqrt{b^{2}-4ac}}{2a} - \frac{b}{2a}
    \end{aligned}
  \end{gather*}
  \begin{gather*}
    \left[x\right]^{1}_{0}
    S = 2\pi\frac{a}{2h}(h - x)\Delta{x}\\
    p = v(h - x)\\
    \begin{aligned}
      P = Sp =& \int v(h - x)2\pi\frac{a}{2h}\Delta{x} \\
      =&2v\pi\frac{a}{2h}\int (h - x)^{2} \Delta{x}
    \end{aligned}
  \end{gather*}
  \begin{gather*}
    \theta = \tan{t} \\
    \begin{aligned}
      & \int \sqrt{\theta^{2} + 1} \\
      =& \int \sqrt{\tan^{2}{t} + 1} \sec^{2}{t} \\
      =& \int \sqrt{\sec^{2}{t}} \sec^{2}{t} = \int \sec^{3}{t} \\
      =& \tan{t}\sec{t} - \int \tan{t}\frac{\sin{t}}{\cos^{2}{t}} \\
      =& \tan{t}\sec{t} - \int \tan^{2}{t}\sec{t} \\
      =& \tan{t}\sec{t} - \int (\sec^{2}{t} - 1)\sec{t} \\
      =& \tan{t}\sec{t} - ( \int \sec^{3}{t} - \int \sec{t} ) \\
      =& \frac{\tan{t}\sec{t} + \int \sec{t}}{2} \qquad \frac{1}{\frac{1 + \sin{t}}{\cos{t}}}\frac{\sin{t} + 1}{\cos^{2}{t}} \\
      =& \frac{\tan{t}\sec{t} + \ln{\sec{t} + \tan{t}}}{2}
    \end{aligned}
  \end{gather*}
\end{document}