\documentclass{article}

\usepackage[margin=1cm]{geometry}
\usepackage{amsmath}
\usepackage{fontspec}
% \setmainfont{texgyretermes-regular.otf}
% \newfontfamily\cjkfont{FandolSong-Regular.otf}
\setmainfont{FandolSong-Regular.otf}

\begin{document}
  % \begin{align}
  %   \begin{aligned}
  %   \end{aligned}
  % \end{align}
  \begin{gather*}
    % \begin{aligned}
      % \int \frac{f'(x)}{F'(x)} dx \\
      % u = F(x) \quad F'(x) = \frac{du}{dx} \\
      % x = G(u) \quad G'(u) = \frac{dx}{du} \\
      % f'(x)dx = f'(G(u))G'(u)du \\
      % \frac{f'(x)}{F'(x)}dx = f'(G(u))G'(u) \frac{1}{F'(x)}du = f'(G(u))G'(u)G'(u)du \\
    % \end{aligned}
  \end{gather*}
  \begin{align}
    \begin{aligned} %拉格朗日中值定理
      & \frac{f\left( a \right) - f\left(b\right)}{a - b} = f'\left( \xi  \right) \\
      & \int \frac{f\left( a \right) - f\left(b\right)}{a - b} - f'\left( x  \right) \\
      =& \frac{f\left( a \right) - f\left(b\right)}{a - b} x - f\left( x \right) + C \\
      =& \frac{f\left( a \right) x - f\left(b\right) x - f\left(x\right) a + f\left(x\right) b}{a - b} + C
    \end{aligned}
  \end{align}
  \begin{gather} %柯西中值定理
    \begin{gathered}
      \frac{f\left( a \right) - f\left(b\right)}{F\left(a\right) - F\left(b\right)} = \frac{f'\left( \xi  \right)}{F'\left( \xi \right)} \\
      ( f(a) - f(b) ) F'(\xi) - ( F(a) - F(b) ) f'(\xi) = 0 \\
      \int ( f(a) - f(b) ) F'(x) - ( F(a) - F(b) ) f'(x) \quad dx \\
      = ( f(a) - f(b) ) F(x) - ( F(a) - F(b) ) f(x)
    \end{gathered}
    % \begin{aligned}
      % & \frac{f'(x)}{F'(x)} = \frac{\Delta{f(x)}}{\Delta{x}} \frac{\Delta{x}}{\Delta{F(x)}} \\
      % & Y = f(x) \quad X = F(x) \\
      % & g(X) = Y \\
      % & g'(x) = \frac{f'(x)}{F'(x)} \\
      % & t = F(x) \quad F'(x) = \frac{\Delta{t}}{\Delta{x}} \quad F^{-1}(t) = \frac{\Delta{x}}{\Delta{t}} \\
      % & \int \frac{f\left( a \right) - f\left(b\right)}{F\left(a\right) - F\left(b\right)} - \frac{f'\left( x \right)}{F'\left( x \right)} \\
      % = & \int \frac{f\left( a \right) - f\left(b\right)}{F\left(a\right) - F\left(b\right)} - g'(X) \\
      % = & \frac{f\left( a \right) - f\left(b\right)}{F\left(a\right) - F\left(b\right)} X - g(X) + C \\
      % = & \frac{f\left( a \right) - f\left(b\right)}{F\left(a\right) - F\left(b\right)} F(x) - f(x) + C \\
      % = & \frac{f\left( a \right) F(x) - f\left(b\right) F(x) - f\left(x\right) F(a) + f\left(x\right) F(b)}{F(a) - F(b)} + C
    % \begin{aligned}
  \end{gather}
  \begin{gather} %洛必达法则
    \begin{gathered}
      x \to x_{0} \Rightarrow  f(x) \to 0 \Rightarrow  F(x) \to 0 \\
      \lim_{x \to x_{0}}\frac{f(x)}{F(x)} = \frac{f'(x_{0})}{F'(x_{0})} \\
      x - \Delta{x} = x_{0} \quad x \to x_0 \Rightarrow \Delta{x} \to 0 \\
      \lim_{x \to x_{0}} \frac{f(x)}{F(x)}
      = \lim_{\Delta{x} \to 0} \frac{f(x_{0} + \Delta{x})}{F(x_{0} + \Delta{x})}
    \end{gathered}
  \end{gather}
  \begin{gather}
    \begin{aligned}
      \lim_{\Delta{x} \to 0}& \frac{\left(x+\Delta{x}\right)^{\frac{a}{b}} - x^{\frac{a}{b}}}{\Delta{x}} \\
      =& x^{\frac{a}{b}} \frac{ \left( 1 + \frac{\Delta{x}}{x} \right)^{\frac{a}{b}} - 1}{\Delta{x}} \\
    \end{aligned} \\
    \begin{aligned}
      \lim_{\Delta{x} \to 0} \frac{\left( 1 + \frac{\Delta{x}}{x} \right)^{\frac{a}{b}} - 1} {\frac{a}{b} \frac{\Delta{x}}{x}} \\
      \left( 1 + \frac{\Delta{x}}{x} \right)^{\frac{x}{\Delta{x}}} &= e \\
      % \log_{\left( 1 + \frac{\Delta{x}}{x} \right)} e &= \frac{x}{\Delta{x}} \\
      % \ln \left( 1 + \frac{\Delta{x}}{x} \right) &= \frac{\Delta{x}}{x} \\
      \lim_{t \to 0} t &= e^{\frac{\Delta{x}}{x} \frac{a}{b}} - 1\\
      \ln \left( t + 1 \right) &= \frac{\Delta{x}}{x} \frac{a}{b} \\
      \frac{e^{\frac{\Delta{x}}{x} \frac{a}{b}} - 1}{\frac{\Delta{x}}{x} \frac{a}{b}} &=
      \frac{t}{ln \left( t + 1 \right)} \\
      &= \frac{1}{\frac{\ln t + 1}{t}}
      % \lim_{\Delta{x} \to 0} \left( 1 + \frac{\Delta{x}}{x} \right)^{\frac{a}{b}} &= e^{\frac{x}{\Delta{x}} \frac{a}{b}}
    \end{aligned}
    \qquad
    \begin{aligned}
      t &= \left(1 + \frac{\Delta{x}}{x} \right)^{\frac{1}{b}} \\
      \Delta{x} &= x \left( t^{b} - 1 \right) \\
      \Delta{x} \to 0 &\Rightarrow t \to 1 \\
      &\lim_{\Delta{x} \to 0} \frac{ \left( 1 + \frac{\Delta{x}}{x} \right)^{\frac{a}{b}} - 1}{\Delta{x}} \\
      = &\lim_{t \to 1} \frac{1}{x} \frac{t^{a} - 1}{t^{b} - 1} \\
      = &\lim_{t \to 1} \frac{1}{x} \frac{a}{b} \frac{t^{a -1}}{t^{b - 1}} \qquad \text{(洛必达法则)} %%
    \end{aligned}
  \end{gather}
\end{document}