\documentclass{article}

\usepackage[margin=1cm]{geometry}
\usepackage{amsmath}
\usepackage{fontspec}
\setmainfont{FandolSong-Regular.otf}

\begin{document}
\begin{gather*}
  \lim_{x \to \infty}\frac{F'(x)}{g'(x)} = l \\
  f'(x) = F'(x) - g'(x)l \\
  \lim_{x \to \infty}\frac{f'(x)}{g'(x)} = 0 \\
  \begin{aligned}
    \frac{f(x_1) - f(x_2)}{g(x_1) - g(x_2)} &= \frac{f'(\xi)}{g'(\xi)} \\
    \frac{\frac{f(x_1)}{g(x_1)} - \frac{f(x_2)}{g(x_1)}}{1 - \frac{g(x_2)}{g(x_1)}} &= \\
    \frac{f(x_1)}{g(x_1)} &= \frac{f'(\xi)}{g'(\xi)}\left(1 - \frac{g(x_2)}{g(x_1)}\right) + \frac{f(x_2)}{g(x_2)} \\
                          &\leq \left\lvert \frac{f'(\xi)}{g'(\xi)} \right\rvert
                             \left\lvert (1 - \frac{g(x_2)}{g(x_1)}) \right\rvert
                             + \left\lvert \frac{f(x_2)}{g(x_2)} \right\rvert
  \end{aligned} \\
  \forall \varepsilon \exists \xi \in (\Delta, +\infty) \cap (x_1, x_2) \\
  \frac{f'(\xi)}{g'(\xi)} < \frac{\varepsilon}{3} \\
  x_1 \in (\Delta, +\infty) \\
  x_2 \in (x_1, +\infty) \\
  \left\lvert\frac{g(x_2)}{g(x_1)}\right\rvert < \frac{1}{2} \\
  \left\lvert\frac{f(x_2)}{g(x_1)}\right\rvert < \frac{\varepsilon}{2} \left(< \frac{1}{2} \right)
\end{gather*}


设：
\[
  \lim_{x \rightarrow x_{0}}{f\left( x \right)}=A
\]

求证：
\[
  \lim_{x \rightarrow x_0}{\frac{f\left( x \right)}{g\left( x \right)}}=\frac{A}{B}
\]

证：
\[
  \lim_{x \rightarrow x_0}{f\left( x \right)}=A \text{则} \forall \quad \varepsilon_1 \exists \delta_1 \text{当} \left| x - x_0 \right|<\delta_1 \text{时} \left| f\left( x \right)-A \right|<\varepsilon_1
\]
\[
  \lim_{x \rightarrow x_0}{g\left( x \right)}=B \text{则} \forall \quad \varepsilon_2 \exists \delta_2 \text{当} \left| x - x_0 \right|<\delta_2 \text{时} \left| f\left( x \right)-B \right|<\varepsilon_2
\]
\begin{align*}
  \left| \frac{f\left( x \right)}{g\left( x \right)}-\frac{A}{B} \right| &= \left| \frac{f\left( x \right)}{g\left( x \right)}-\frac{A}{B}-\frac{A}{g\left( x \right)}+\frac{A}{g\left(x\right)} \right| \\
  & =\left| \frac{f\left( x \right)-A}{g\left( x \right)}-\frac{A\left( g\left( x \right)-B \right)}{Bg\left( x \right)} \right| \\
  & =\left| \frac{B\left( f\left( x \right)-A \right)-A\left( g\left( x \right)-B \right)}{Bg\left( x \right)} \right| \\
  & \leq\frac{\left| B \right|\left| f\left( x \right)-A \right|+\left| A \right|\left| g\left(x\right)-B \right|}{\left|B\right|\left|g\left(x\right)\right|} \tag*{(1)}\label{1} \\
\end{align*}
\[
  \text{因为} \exists \delta_3 \text{当} \left|x-x_0\right|<\delta_3 \text{时} \left| g\left(x\right)\right|>\left|\frac{B}{2}\right| \quad \left|\frac{1}{g\left(x\right)}\right|<\left|\frac{2}{B}\right|
\]
\[
  \ref{1} < \frac{\left|B\right|\left|f\left(x\right)-A\right|+\left|A\right|\left|g\left(x\right)-B\right|}{\left|B\right|}\times\left|\frac{2}{B}\right|
\]
\[
  \forall \varepsilon \text{当} \varepsilon_1=\frac{\left|B\right|\varepsilon}{4} \quad \varepsilon_2=\frac{B^{2}\varepsilon}{4\left|A\right|}
\]
\[
  \text{取} \delta=min\left(\delta_1,\delta_2,\delta_3\right) \text{取} \left|x-x_0\right|<\delta \text{时} \left|\frac{f\left(x\right)}{g\left(x\right)}-\frac{A}{B}\right|<\varepsilon
\]
\end{document}