\documentclass{article}

\usepackage[margin=1cm]{geometry}
\usepackage{amsmath}
\usepackage{fontspec}
\setmainfont{FandolSong-Regular.otf}

\newcommand\F[2]{\frac{#1}{#2}}
\begin{document}
  \begin{gather*}
    \begin{aligned}
      & \lim_{\Delta x \to 0}
        \left(
          \left(
            1+\frac{\Delta x}{x}
          \right)^{\frac{1}{\frac{\Delta x}{x}}}
        \right)^{\left(\frac{\Delta x}{x}\right)u}
      -1 \\
      = & \lim_{\Delta x \to 0}
        e^{\left(\frac{\Delta x}{x}\right)u} -1
    \end{aligned} \\
    t = e^{\frac{\Delta x}{x}}u-1 \\
    \Delta x \to 0 t \to 0 \\
    \frac{\Delta x}{x}u=ln(t+1) \\
    \frac{\ln(t+1)}{t} = 1
  \end{gather*}
  \begin{gather*}
    \lim_{\Delta x \to 0}
    \frac{\left(1 + \frac{\Delta x}{x}\right)^n - 1}{n\frac{\Delta x}{x}}
  \end{gather*}
  \begin{gather*}
    T m \omega r s \\
    T \omega r m \\
    T \sin{\omega s} m \\
    v = \omega\frac{d\pi}{2\pi} \\
    U = 2 B l \omega\frac{d\pi}{2\pi} \sin{\omega t} \\
    \begin{aligned}
      & \int_0^T \frac{(Bl \omega d \sin{\omega t})^2}{R} \Delta t \\
      = & \frac{(Bl\omega d)^2}{R} \int_{0}^{T} \sin^2 \omega t \Delta t
    \end{aligned}
    % \begin{aligned}
    %   & \int_0^T \frac{Bl \omega d \sin{\omega t}}{R} \Delta t \\
    %   = & \frac{Bl\omega d}{R} \int_{0}^{T} \sin \omega t \Delta t \\
    %   = & \frac{Bl\omega d}{R} -\frac{1}{\omega} \int_{0}^{T} \omega \times -\sin \omega t \Delta t \\
    %   = & \frac{Bl\omega d}{R} \frac{1}{\omega} \left[ \cos{\omega t} \right]_0^T
    % \end{aligned}
  \end{gather*}
  \begin{gather*}
    Wb = Tm^2 \\
    T = \frac{N}{Am} \\
    A = \frac{q}{s} \\
    N = Tqm/s \\
    N = TAm \\
    V = J/q \\
    J = Nm
  \end{gather*}
  \begin{gather*}
    U_e + U_{r_1} = I_1(R_e + R_{r_1}) \\
    U_e + U_{r_2} = I_2(R_e + R_{r_2}) \\
    R_e = \frac{( U_{r_1} - U_{r_2} ) - ( I_1 R_{r_1} - I_2 R_{r_2} )}{I_1 - I_2}
  \end{gather*}
  \begin{gather*}
    R_l \quad R_0 \quad R_A \quad R_R \\
    \frac{1}{R_D} = \frac{1}{R_A} + \frac{1}{R_R} \\
    R_l = R_0 + R_D \\
    U = IR_l \\
    I = \frac{U}{R_l}
  \end{gather*}
  \begin{gather*}
    \frac{Uql^2}{dmv ^22}
  \end{gather*}
  \begin{gather*}
    l_{n} = Tv_{n} \\
    v_{n} = \sqrt{\frac{2nW}{m}}
  \end{gather*}
  \begin{gather*}
    W = FS \\
    a = \frac{F}{m} \\
    \Delta v = at \\
    t = \frac{S}{v_{0} + \frac{\Delta v}{2}} \\
    \begin{aligned}
      \Delta v &= \frac{F}{m} \frac{S}{v_{0} + \frac{\Delta v}{2}} \\
      &= \frac{W}{m(v_{0} + \frac{1}{2}\Delta v)} \\
      v_{0}\Delta v + \frac{1}{2}\Delta v^{2} &= \frac{W}{m}
    \end{aligned} \\
    t = \frac{2S}{v_{1} + v_{0}} \\
    \begin{aligned}
      \Delta v &= \frac{2W}{m(v_{1} + v_{0})} \\
      % &= \sqrt{\frac{2W}{m}}
    \end{aligned}
  \end{gather*}
  \begin{gather*}
    F = Bqv = \frac{mv^2}{r} \\
    r = \frac{mv}{Bq} \\
    t = \frac{2\pi r}{v} = \frac{2\pi}{v} \frac{mv}{Bq}
  \end{gather*}
  \begin{gather*}
    U \quad B \quad q \quad m \quad s \\
    a = \F{Uq}{sm} \\
    F = m\F{v^2}{r} = ma^2r = Bqv \\
    r = \F{mv^2}{Bqv} = \F{mv}{Bq} \\
    t = \F{2\pi}{a} = \F{2\pi r}{v} = \F{2\pi m}{Bq}
  \end{gather*}
  \begin{gather*}
    Bvq = F = \F{mv^2}{r} \\
    Bq = \F{mv}{r} \\
    s = \F{at^2}{2} = \F{vt}{2} \\
    Uq = Fs = ams = \F{(at)^2m}{2} = \F{1}{2}v^2m \\
    v = \sqrt{\F{2Uq}{m}} \\
    Bq = \F{m\sqrt{\F{2Uq}{m}}}{r}
  \end{gather*}
\end{document}